theories/Core/Semantic/Readback/Lemmas.v
@@ -8,20 +8,20 @@ Import Domain_Notations.
 
 Section functional_read.
   Lemma functional_read {P : PtsSig} :
-    (forall i (m : domain_nf P) M1,
-        {{ Rnf m in i ↘ M1 }} ->
+    (forall (Δ : gctx P) i m M1,
+        {{ Δ ▶ Rnf m in i ↘ M1 }} ->
         forall M2,
-          {{ Rnf m in i ↘ M2 }} ->
+          {{ Δ ▶ Rnf m in i ↘ M2 }} ->
           M1 = M2) /\
-      (forall i (e : domain_ne P) E1,
-          {{ Rne e in i ↘ E1 }} ->
+      (forall (Δ : gctx P) i e E1,
+          {{ Δ ▶ Rne e in i ↘ E1 }} ->
           forall E2,
-            {{ Rne e in i ↘ E2 }} ->
+            {{ Δ ▶ Rne e in i ↘ E2 }} ->
             E1 = E2) /\
-      (forall i (a : domain P) A1,
-          {{ Rtyp a in i ↘ A1 }} ->
+      (forall (Δ : gctx P) i a A1,
+          {{ Δ ▶ Rtyp a in i ↘ A1 }} ->
           forall A2,
-            {{ Rtyp a in i ↘ A2 }} ->
+            {{ Δ ▶ Rtyp a in i ↘ A2 }} ->
             A1 = A2).
   Proof with (functional_eval_rewrite_clear; f_equal; solve [eauto]) using.
     apply read_mut_ind; intros.
@@ -47,25 +47,25 @@ Section functional_read.
       reflexivity.
   Qed.
 
-  Corollary functional_read_nf {P : PtsSig} : forall i (v : domain_nf P) V1 V2,
-      {{ Rnf v in i ↘ V1 }} ->
-      {{ Rnf v in i ↘ V2 }} ->
+  Corollary functional_read_nf {P : PtsSig} : forall (Δ : gctx P) i v V1 V2,
+      {{ Δ ▶ Rnf v in i ↘ V1 }} ->
+      {{ Δ ▶ Rnf v in i ↘ V2 }} ->
       V1 = V2.
   Proof.
     pose proof @functional_read P; firstorder.
   Qed.
 
-  Lemma functional_read_ne {P : PtsSig} : forall i (e : domain_ne P) E1 E2,
-      {{ Rne e in i ↘ E1 }} ->
-      {{ Rne e in i ↘ E2 }} ->
+  Lemma functional_read_ne {P : PtsSig} : forall (Δ : gctx P) i e E1 E2,
+      {{ Δ ▶ Rne e in i ↘ E1 }} ->
+      {{ Δ ▶ Rne e in i ↘ E2 }} ->
       E1 = E2.
   Proof.
     pose proof @functional_read P; firstorder.
   Qed.
 
-  Lemma functional_read_typ {P : PtsSig} : forall i (a : domain P) A1 A2,
-      {{ Rtyp a in i ↘ A1 }} ->
-      {{ Rtyp a in i ↘ A2 }} ->
+  Lemma functional_read_typ {P : PtsSig} : forall (Δ : gctx P) i a A1 A2,
+      {{ Δ ▶ Rtyp a in i ↘ A1 }} ->
+      {{ Δ ▶ Rtyp a in i ↘ A2 }} ->
       A1 = A2.
   Proof.
     pose proof @functional_read P; firstorder.
@@ -78,11 +78,11 @@ Hint Resolve functional_read_nf functional_read_ne functional_read_typ : mcpts.
 Ltac functional_read_rewrite_clear1 :=
   let tactic_error o1 o2 := fail 3 "functional_read equality between" o1 "and" o2 "cannot be solved by mauto" in
   match goal with
-  | H1 : {{ Rnf ^?m in ?s ↘ ^?M1 }}, H2 : {{ Rnf ^?m in ?s ↘ ^?M2 }} |- _ =>
+  | H1 : {{ Δ ▶ Rnf ^?m in ?s ↘ ^?M1 }}, H2 : {{ Δ ▶ Rnf ^?m in ?s ↘ ^?M2 }} |- _ =>
       clean replace M2 with M1 by first [solve [mauto 2] | tactic_error M2 M1]; clear H2
-  | H1 : {{ Rne ^?m in ?s ↘ ^?M1 }}, H2 : {{ Rne ^?m in ?s ↘ ^?M2 }} |- _ =>
+  | H1 : {{ Δ ▶ Rne ^?m in ?s ↘ ^?M1 }}, H2 : {{ Δ ▶ Rne ^?m in ?s ↘ ^?M2 }} |- _ =>
       clean replace M2 with M1 by first [solve [mauto 2] | tactic_error M2 M1]; clear H2
-  | H1 : {{ Rtyp ^?m in ?s ↘ ^?M1 }}, H2 : {{ Rtyp ^?m in ?s ↘ ^?M2 }} |- _ =>
+  | H1 : {{ Δ ▶ Rtyp ^?m in ?s ↘ ^?M1 }}, H2 : {{ Δ ▶ Rtyp ^?m in ?s ↘ ^?M2 }} |- _ =>
       clean replace M2 with M1 by first [solve [mauto 2] | tactic_error M2 M1]; clear H2
   end.
 Ltac functional_read_rewrite_clear := repeat functional_read_rewrite_clear1.
